SStructTT/SStruct/Runtime/Preservation0.lean
@@ -174,6 +174,12 @@ lemma Resolved.preservation0X {H1 H2 H3 H3' : Heap Srt} {a b c c' A} :
       . constructor <;> assumption
       . assumption
     . assumption
+  case exf wf im tyA tym =>
+    subst_vars
+    exact (Logical.Typed.bot_not_derivable tym).elim
+  case exf_drop mrg tyA tym ern erb ihn ihb =>
+    subst_vars
+    exact (Logical.Typed.bot_not_derivable tym).elim
   case drop m m' n n' A B s mrg lw h erm ern ihm ihn =>
     subst_vars; cases mrg; cases rs
     case drop H1' H2' m m' h1 mrg1 rsm rsn =>
