SStructTT/SStruct/Runtime/Preservation1.lean
@@ -418,6 +418,12 @@ lemma Resolved.preservation1X {H1 H2 H3 H3' : Heap Srt} {a b c c' A} :
         assumption
         assumption
       . assumption
+  case exf wf tyA tym =>
+    subst_vars
+    exact (Logical.Typed.bot_not_derivable tym).elim
+  case exf_drop mrg tyA tym ern erb ihn ihb =>
+    subst_vars
+    exact (Logical.Typed.bot_not_derivable tym).elim
   case drop A B s mrg lw h erm ern ihm ihn =>
     subst_vars; cases mrg; cases rs
     case drop => cases st
